src/Iris/Proofmode.lean
@@ -2,6 +2,7 @@ import Iris.Proofmode.Classes
 import Iris.Proofmode.Display
 import Iris.Proofmode.Environments
 import Iris.Proofmode.Expr
+import Iris.Proofmode.InputPatterns
 import Iris.Proofmode.Instances
 import Iris.Proofmode.Tactics
 import Iris.Proofmode.Theorems
